**logical equivilents**
- //p <-> p
- P or Q <-> Q or P
- P and Q <-> Q and P
- P or (Q and R) <-> (P or Q) and (P or R)
  - X * (Y + Z) = X * Y + X * Z
- P and (Q or R) <-> (P and Q) or (Q and R)
  - X + (Y * Z) = ? missed it

**negate and simplify**
- P -> W <-> not P * Q
- not (P -> Q) <-> P and not Q
- not (P or Q) <-> not P and not Q
  - De Morgan's Law
- not (P and Q) <-> not P or not Q

When you simplify:
- negation over variables only, no expressions.
- when you negate it you just put a negate on the outside
